transformation/Sitpn2HVhdlTypes.v
@@ -60,8 +60,8 @@ Section CompileTimeTypes.
 
   Inductive Sitpn2HVhdlMap : Type :=
     MkS2HMap {
-        p2pcomp : list (P sitpn * ident);
-        t2tcomp : list (T sitpn * ident);
+        p2pci : list (P sitpn * ident);
+        t2tci : list (T sitpn * ident);
         a2out   : list (A sitpn * ident);
         f2out   : list (F sitpn * ident);
         c2in    : list (C sitpn * ident);
@@ -124,8 +124,8 @@ Arguments finfos {sitpn}.
 
 (* Set implicit arguments for Sitpn2HVhdlMap *)
 
-Arguments p2pcomp {sitpn}.
-Arguments t2tcomp {sitpn}.
+Arguments p2pci {sitpn}.
+Arguments t2tci {sitpn}.
 Arguments a2out {sitpn}.
 Arguments f2out {sitpn}.
 Arguments c2in {sitpn}.
@@ -245,41 +245,41 @@ Section CompileTimeStateOpers.
     (* Sets the couple [(a, id)] in the [a2out] field of [γ]. *)
     let a2out' := setv Aeqdec a id (a2out γ) in
     (* Updates the new archictecture. *)
-    set_binder (MkS2HMap sitpn (p2pcomp γ) (t2tcomp γ) a2out' (f2out γ) (c2in γ)).
+    set_binder (MkS2HMap sitpn (p2pci γ) (t2tci γ) a2out' (f2out γ) (c2in γ)).
 
   Definition bind_function (f : F sitpn) (id : ident) :=
     do γ <- get_binder;
     (* Sets the couple [(f, id)] in the [f2out] field of [γ]. *)
     let f2out' := setv Feqdec f id (f2out γ) in
     (* Updates the new archictecture. *)
-    set_binder (MkS2HMap sitpn (p2pcomp γ) (t2tcomp γ) (a2out γ) f2out' (c2in γ)).
+    set_binder (MkS2HMap sitpn (p2pci γ) (t2tci γ) (a2out γ) f2out' (c2in γ)).
 
   Definition bind_condition (c : C sitpn) (id : ident) :=
     do γ <- get_binder;
     (* Sets the couple [(c, id)] in the [c2in] field of [γ]. *)
     let c2in' := setv Ceqdec c id (c2in γ) in
     (* Updates the new archictecture. *)
-    set_binder (MkS2HMap sitpn (p2pcomp γ) (t2tcomp γ) (a2out γ) (f2out γ) c2in').
+    set_binder (MkS2HMap sitpn (p2pci γ) (t2tci γ) (a2out γ) (f2out γ) c2in').
 
   Definition bind_place (p : P sitpn) (id : ident) :=
     do γ <- get_binder;
-    (* Sets the couple [(p, id)] in the [p2pcomp] field of [γ]. *)
-    let p2pcomp' := setv Peqdec p id (p2pcomp γ) in
+    (* Sets the couple [(p, id)] in the [p2pci] field of [γ]. *)
+    let p2pci' := setv Peqdec p id (p2pci γ) in
     (* Updates the new archictecture. *)
-    set_binder (MkS2HMap sitpn p2pcomp' (t2tcomp γ) (a2out γ) (f2out γ) (c2in γ)).
+    set_binder (MkS2HMap sitpn p2pci' (t2tci γ) (a2out γ) (f2out γ) (c2in γ)).
 
   Definition bind_transition (t : T sitpn) (id : ident) :=
     do γ <- get_binder;
-    (* Sets the couple [(t, id)] in the [t2tcomp] field of [γ]. *)
-    let t2tcomp' := setv Teqdec t id (t2tcomp γ) in
+    (* Sets the couple [(t, id)] in the [t2tci] field of [γ]. *)
+    let t2tci' := setv Teqdec t id (t2tci γ) in
     (* Updates the new architecture. *)
-    set_binder (MkS2HMap sitpn (p2pcomp γ) t2tcomp' (a2out γ) (f2out γ) (c2in γ)).
+    set_binder (MkS2HMap sitpn (p2pci γ) t2tci' (a2out γ) (f2out γ) (c2in γ)).
 
   Definition get_pci_id_from_binder (p : P sitpn) :=
-    do γ <- get_binder; getv Peqdec p (p2pcomp γ).
+    do γ <- get_binder; getv Peqdec p (p2pci γ).
 
   Definition get_tci_id_from_binder (t : T sitpn) :=
-    do γ <- get_binder; getv Teqdec t (t2tcomp γ).
+    do γ <- get_binder; getv Teqdec t (t2tci γ).
   
   (** *** Operations for beh *)
 
