transformation/proofs/GenerateInterconnectionsFacts.v
@@ -106,8 +106,7 @@ Section ConnToOutputTcisFacts.
           by (rewrite <- eq_beh in InCs10_bis, InCs10; eapply get_comp_uniq_comp; eauto).
         injection eq_comp; auto.
       + (* CASE [id__c <> x1] *)
-        destruct 1 as [ g' [ i' [ o' InCs10 ] ] ];
-          do 3 eexists; eauto with put_comp.
+        destruct 1 as [ g' [ i' [ o' InCs10 ] ] ]; do 3 eexists; eauto with put_comp.
   Qed.
 
   Lemma conn_to_output_tcis_pci_ex_inv :
@@ -115,13 +114,13 @@ Section ConnToOutputTcisFacts.
            {s : Sitpn2HVhdlState sitpn} {v s' p},
       connect_to_output_tcis pinfo i o s = OK v s' ->
       (exists id__p g__p i__p o__p,
-          InA Pkeq (p, id__p) (p2pcomp (γ s))
+          InA Pkeq (p, id__p) (p2pci (γ s))
           /\ InCs (cs_comp id__p Petri.place_entid g__p i__p o__p) (beh s)) ->
       (exists id__p g__p i__p o__p,
-          InA Pkeq (p, id__p) (p2pcomp (γ s'))
+          InA Pkeq (p, id__p) (p2pci (γ s'))
           /\ InCs (cs_comp id__p Petri.place_entid g__p i__p o__p) (beh s')).
   Proof.
-    destruct 2 as [ id__p [ g__p [ i__p [ o__p [ InA_p2pcomp InCss ] ] ] ] ].
+    destruct 2 as [ id__p [ g__p [ i__p [ o__p [ InA_p2pci InCss ] ] ] ] ].
     exists id__p.
     cut (exists g__p i__p o__p, InCs (cs_comp id__p Petri.place_entid g__p i__p o__p) (beh s')).
     intros InCs_ex; destruct InCs_ex as [ g__p' [ i__p' [ o__p' InCss' ] ] ].
@@ -141,10 +140,10 @@ Section GenInterFacts.
       generate_interconnections s = OK v s' ->
       NoDup (get_cids (beh s)) ->
       (exists id__p g__p i__p o__p,
-          InA Pkeq (p, id__p) (p2pcomp (γ s))
+          InA Pkeq (p, id__p) (p2pci (γ s))
           /\ InCs (cs_comp id__p Petri.place_entid g__p i__p o__p) (beh s)) ->
       (exists id__p g__p i__p o__p,
-          InA Pkeq (p, id__p) (p2pcomp (γ s'))
+          InA Pkeq (p, id__p) (p2pci (γ s'))
           /\ InCs (cs_comp id__p Petri.place_entid g__p i__p o__p) (beh s')).
   Proof.  
     intros *; intros H; pattern s, s'.
