transformation/proofs/GeneratePortsFacts.v
@@ -3,36 +3,211 @@
 Require Import String.
 Require Import common.CoqLib.
 Require Import common.StateAndErrorMonad.
-Require Import common.StateAndErrorMonadTactics.
-Require Import common.ListMonadFacts.
-Require Import common.ListMonadTactics.
+Require Import common.proofs.StateAndErrorMonadTactics.
+Require Import common.proofs.ListMonadFacts.
+Require Import common.proofs.ListMonadTactics.
 Require Import common.ListPlus.
-Require Import common.SetoidListFacts.
+Require Import common.proofs.SetoidListFacts.
 
 Require Import sitpn.SitpnLib.
 
 Require Import hvhdl.AbstractSyntax.
 
 Require Import transformation.Sitpn2HVhdl.
-Require Import transformation.GenerateArchitectureFacts.
+Require Import transformation.Sitpn2HVhdlUtils.
+Require Import transformation.proofs.SInvTactics.
+Require Import transformation.proofs.Sitpn2HVhdlUtilsFacts.
 
 (** ** Facts about Action Port Generation *)
 
 Section GenActionPorts.
-    
+
+  Lemma gen_aports_inv_p2pci :
+    forall {sitpn s v s'},
+      generate_action_ports_and_ps sitpn s = OK v s' ->
+      p2pci (γ s) = p2pci (γ s').
+  Proof. intros * EQ; pattern s, s'; solve_sinv_pattern. Qed.
+
+  Lemma gen_aports_inv_t2tci :
+    forall {sitpn s v s'},
+      generate_action_ports_and_ps sitpn s = OK v s' ->
+      t2tci (γ s) = t2tci (γ s').
+  Proof. intros * EQ; pattern s, s'; solve_sinv_pattern. Qed.
+
+  Lemma gen_aports_inv_lofPs :
+    forall {sitpn s v s'},
+      generate_action_ports_and_ps sitpn s = OK v s' ->
+      lofPs s = lofPs s'.
+  Proof. intros * EQ; pattern s, s'; solve_sinv_pattern. Qed.
+
+  Lemma gen_aports_inv_lofTs :
+    forall {sitpn s v s'},
+      generate_action_ports_and_ps sitpn s = OK v s' ->
+      lofTs s = lofTs s'.
+  Proof. intros * EQ; pattern s, s'; solve_sinv_pattern. Qed.
+
+  Lemma gen_aports_pci_ex :
+    forall {sitpn s v s' p},
+      generate_action_ports_and_ps sitpn s = OK v s' ->
+      (exists id__p g__p i__p o__p,
+          InA Pkeq (p, id__p) (p2pci (γ s))
+          /\ InCs (cs_comp id__p Petri.place_entid g__p i__p o__p) (beh s)) -> 
+      (exists id__p g__p i__p o__p,
+          InA Pkeq (p, id__p) (p2pci (γ s'))
+          /\ InCs (cs_comp id__p Petri.place_entid g__p i__p o__p) (beh s')).
+  Proof. intros * EQ; pattern s, s'; solve_sinv_pattern.
+         minv EQ3; cbn.
+         intros [ id__p [ g__p [ i__p [ o__p [ InA_p2pci InCs_ ] ] ] ] ];
+           do 4 eexists; split; [ | right ]; eauto.
+  Qed.
+  
 End GenActionPorts.
 
 (** ** Facts about Function Port Generation *)
 
 Section GenFunPorts.
   
+  Lemma gen_fports_inv_p2pci :
+    forall {sitpn s v s'},
+      generate_fun_ports_and_ps sitpn s = OK v s' ->
+      p2pci (γ s) = p2pci (γ s').
+  Proof. intros * EQ; pattern s, s'; solve_sinv_pattern. Qed.
+
+  Lemma gen_fports_inv_t2tci :
+    forall {sitpn s v s'},
+      generate_fun_ports_and_ps sitpn s = OK v s' ->
+      t2tci (γ s) = t2tci (γ s').
+  Proof. intros * EQ; pattern s, s'; solve_sinv_pattern. Qed.
+
+  Lemma gen_fports_inv_lofPs :
+    forall {sitpn s v s'},
+      generate_fun_ports_and_ps sitpn s = OK v s' ->
+      lofPs s = lofPs s'.
+  Proof. intros * EQ; pattern s, s'; solve_sinv_pattern. Qed.
+
+  Lemma gen_fports_inv_lofTs :
+    forall {sitpn s v s'},
+      generate_fun_ports_and_ps sitpn s = OK v s' ->
+      lofTs s = lofTs s'.
+  Proof. intros * EQ; pattern s, s'; solve_sinv_pattern. Qed.   
+
+  Lemma gen_fports_pci_ex :
+    forall {sitpn s v s' p},
+      generate_fun_ports_and_ps sitpn s = OK v s' ->
+      (exists id__p g__p i__p o__p,
+          InA Pkeq (p, id__p) (p2pci (γ s))
+          /\ InCs (cs_comp id__p Petri.place_entid g__p i__p o__p) (beh s)) -> 
+      (exists id__p g__p i__p o__p,
+          InA Pkeq (p, id__p) (p2pci (γ s'))
+          /\ InCs (cs_comp id__p Petri.place_entid g__p i__p o__p) (beh s')).
+  Proof. intros * EQ; pattern s, s'; solve_sinv_pattern.
+         minv EQ3; cbn.
+         intros [ id__p [ g__p [ i__p [ o__p [ InA_p2pci InCs_ ] ] ] ] ];
+           do 4 eexists; split; [ | right ]; eauto.
+  Qed.
   
 End GenFunPorts.
 
 (** ** Facts about Condition Port Generation *)
 
 Section GenCondPorts.
+
+  Lemma gen_cports_inv_p2pci :
+    forall {sitpn s v s'},
+      generate_and_connect_cond_ports sitpn s = OK v s' ->
+      p2pci (γ s) = p2pci (γ s').
+  Proof. intros * EQ; pattern s, s'; solve_sinv_pattern. Qed.
+
+  Lemma gen_cports_inv_t2tci :
+    forall {sitpn s v s'},
+      generate_and_connect_cond_ports sitpn s = OK v s' ->
+      t2tci (γ s) = t2tci (γ s').
+  Proof. intros * EQ; pattern s, s'; solve_sinv_pattern. Qed.
+  
+  Lemma gen_cports_inv_lofPs :
+    forall {sitpn s v s'},
+      generate_and_connect_cond_ports sitpn s = OK v s' ->
+      lofPs s = lofPs s'.
+  Proof. intros * EQ; pattern s, s'; solve_sinv_pattern. Qed.
+
+  Lemma gen_cports_inv_lofTs :
+    forall {sitpn s v s'},
+      generate_and_connect_cond_ports sitpn s = OK v s' ->
+      lofTs s = lofTs s'.
+  Proof. intros * EQ; pattern s, s'; solve_sinv_pattern. Qed.
+  
+  Lemma gen_cports_pci_ex :
+    forall {sitpn s v s' p},
+      generate_and_connect_cond_ports sitpn s = OK v s' ->
+      (exists id__p g__p i__p o__p,
+          InA Pkeq (p, id__p) (p2pci (γ s))
+          /\ InCs (cs_comp id__p Petri.place_entid g__p i__p o__p) (beh s)) -> 
+      (exists id__p g__p i__p o__p,
+          InA Pkeq (p, id__p) (p2pci (γ s'))
+          /\ InCs (cs_comp id__p Petri.place_entid g__p i__p o__p) (beh s')).
+  Proof. intros * EQ; pattern s, s'; solve_sinv_pattern.
+         minv EQ13.
+         intros [ id__p [ g__p [ i__p [ o__p [ InA_p2pci InCss7 ] ] ] ] ].
+         exists id__p.
+         (* 2 CASES [id__p = x2] or [id__p <> x2] *)
+         destruct (Nat.eq_dec id__p x2) as [ eq_ | neq_ ].
+         + (* CASE [id__p = x2] *)
+           subst.
+           exists g, x4, o; split; [ assumption | ].
+           cut (Petri.place_entid = i0); [ intros eq_id__e; subst; eapply put_comp_aux_InCs; eauto | ].
+           assert (eq_beh : beh s3 = beh s6) by (pattern s3, s6; mend_sinv).
+           assert (InCss6 : InCs (cs_comp x2 i0 g i o) (beh s6))
+             by (rewrite <- eq_beh; eapply get_comp_InCs; eauto).
+           erewrite <- put_comp_aux_inv_state in InCss7; eauto.
+           assert (eq_comp : cs_comp x2 Petri.place_entid g__p i__p o__p = cs_comp x2 i0 g i o)
+             by (rewrite <- eq_beh in InCss7, InCss6; eapply get_comp_uniq_comp; eauto).
+           injection eq_comp; auto.
+         + (* CASE [id__p <> x2] *)
+           erewrite <- put_comp_aux_inv_state in InCss7; eauto.
+           do 3 eexists; eauto with put_comp.
+  Qed.
   
 End GenCondPorts.
 
 (** ** Facts about Port Generation Function *)
+
+Lemma gen_ports_inv_p2pci :
+  forall {sitpn s v s'},
+    @generate_ports sitpn s = OK v s' ->
+    p2pci (γ s) = p2pci (γ s').
+Proof. intros * EQ; pattern s, s'; solve_sinv_pattern. Qed.
+
+Lemma gen_ports_inv_t2tci :
+  forall {sitpn s v s'},
+    @generate_ports sitpn s = OK v s' ->
+    t2tci (γ s) = t2tci (γ s').
+Proof. intros * EQ; pattern s, s'; solve_sinv_pattern. Qed.
+
+Lemma gen_ports_inv_lofPs :
+  forall {sitpn s v s'},
+    @generate_ports sitpn s = OK v s' ->
+    lofPs s = lofPs s'.
+Proof. intros * EQ; pattern s, s'; solve_sinv_pattern. Qed.
+
+Lemma gen_ports_inv_lofTs :
+  forall {sitpn : Sitpn} {s : Sitpn2HVhdlState sitpn} {v : unit}
+         {s' : Sitpn2HVhdlState sitpn},
+    generate_ports s = OK v s' -> lofTs s = lofTs s'.
+Proof. intros * EQ; pattern s, s'; solve_sinv_pattern. Qed.
+
+Lemma gen_ports_pci_ex :
+  forall (sitpn : Sitpn) (s : Sitpn2HVhdlState sitpn) v s' p,
+    generate_ports s = OK v s' ->
+    (exists id__p g__p i__p o__p,
+        InA Pkeq (p, id__p) (p2pci (γ s))
+        /\ InCs (cs_comp id__p Petri.place_entid g__p i__p o__p) (beh s)) -> 
+    (exists id__p g__p i__p o__p,
+        InA Pkeq (p, id__p) (p2pci (γ s'))
+        /\ InCs (cs_comp id__p Petri.place_entid g__p i__p o__p) (beh s')).
+Proof. intros * EQ pci_ex; monadInv EQ.
+       eapply gen_cports_pci_ex; eauto;
+         eapply gen_fports_pci_ex; eauto;
+         eapply gen_aports_pci_ex; eauto.
+Qed.
+
+
