transformation/proofs/Sitpn2HVhdlInvs.v
@@ -1,3 +1,1 @@
-Require Export transformation.proofs.GenerateInfosInvs.
-Require Export transformation.proofs.GeneratePortsInvs.
 Require Export transformation.proofs.GenerateHVhdlInvs.
